src/compiler/meta/OCL_compiler_meta_UML_extended.thy
@@ -86,4 +86,8 @@ datatype ocl_def_pre_post = OclDefPP
                               string (* pre *)
                               string (* post *)
 
+subsection{* ... *}
+
+definition "ocl_instance_single_empty = \<lparr> Inst_name = \<langle>''''\<rangle>, Inst_ty = \<langle>''''\<rangle>, Inst_attr = OclAttrNoCast [] \<rparr>"
+
 end
